# 1

## a)

| a\bc | 00   | 01   | 11   | 10   |
| ---- | ---- | ---- | ---- | ---- |
| 0    | m0   | m1   | m3   |      |
| 1    |      |      | m3   |      |

$$
\begin{align*}
A'B'C'+A'B'C+A'BC+ABC
&=A'B'(C+C')+BC(A'+A)\\
&=A'B'+BC
\end{align*}
$$

## b)

| A\BC | 00   | 01   | 11   | 10   |
| ---- | ---- | ---- | ---- | ---- |
| 0    | m0   | m1   |      | m2   |
| 1    | m4   | m5   |      |      |

$$
\begin{align*}
A'B'C'+A'B'C+A'BC'+AB'C'+AB'C
&=B(A'+A)(C'+C)+A'C'(B+B')\\
&=B'+A'C'
\end{align*}
$$

## c)

| x\y  | 0    | 1    |
| ---- | ---- | ---- |
| 0    | m0   | m1   |
| 1    |      | m3   |

$$
\begin{align*}
x'y'+xy+x'y
&=x'(y+y')+y(x'+x)\\
&=x'+y
\end{align*}
$$

# 2

## a)

| X\YZ | 00   | 01   | 11   | 10   |
| ---- | ---- | ---- | ---- | ---- |
| 0    |      |      | m3   |      |
| 1    | m4   |      | m7   | m6   |

$$
\begin{align*}
F(X,Y,Z)
&=\sum m(3,4,6,7)\\
&=YZ(X+X')+XZ'(Y+Y')\\
&=YZ+XZ'
\end{align*}
$$

## b)

| X\YZ | 00   | 01   | 11   | 10   |
| ---- | ---- | ---- | ---- | ---- |
| 0    | m0   |      |      | m2   |
| 1    | m4   | m5   |      | m6   |

$$
\begin{align*}
F(X,Y,Z)
&=\sum m(0,2,4,5,6)\\
&=Z(X+X')(Y+Y')+XY'(Z+Z')\\
&=Z+XY'
\end{align*}
$$

## c)

| AB\CD | 00   | 01   | 11   | 10   |
| ----- | ---- | ---- | ---- | ---- |
| 00    | m0   | m1   |      | m2   |
| 01    | m4   | m5   |      | m6   |
| 11    | m12  | m13  |      | m14  |
| 10    | m8   | m9   |      |      |


$$
\begin{align*}
  F(A,B,C,D) &= \sum m(0,1,2,4,5,6,8,9,12,13,14) \\
    &= C'(A+A')(B+B')(C+C')+A'D'(B+B')(C+C')+BD'(A+A')(C+C')* \\
    &= C+A'D'+BD'
\end{align*}
$$

# 3

## a)

| A\BC | 00   | 01   | 11   | 10   |
| ---- | ---- | ---- | ---- | ---- |
| 0    |      |      |      |      |
| 1    |      | m5   | m7   | m6   |

$$
\begin{align*}
AB+AB'C+ABC 
&=\sum m(5,6,7)\\
&=AC(B+B')+AB(C+C')\\
&=AC+AB
\end{align*}
$$

## b)

| A\BC | 00   | 01   | 11   | 10   |
| ---- | ---- | ---- | ---- | ---- |
| 0    |      |      | m3   |      |
| 1    | m4   | m5   | m7   | m6   |

$$
\begin{align*}
A+BC
&=\sum m(3,4,5,6,7)\\
&=A(B+B')(C+C')+BC(A+A')\\
&=A+BC
\end{align*}
$$

## c)

| AB\CD | 00   | 01   | 11   | 10   |
| ----- | ---- | ---- | ---- | ---- |
| 00    |      |      |      |      |
| 01    |      | m5   |      | m6   |
| 11    |      | m13  |      | m14  |
| 10    |      | m9   |      | m10  |

$$
\begin{align*}
AB'C'D+ACD'+BC'D+A'BCD'
&=\sum m(5,6,9,10,13,14)\\
&=BC'D(A+A')+AC'D(B+B')+BCD'(A+A')+ACD'(B+B')\\
&=BCD'+AC'D+BCD'+ACD'
\end{align*}
$$

## d)

| AB\CD |      |      |      |      |
| ----- | ---- | ---- | ---- | ---- |
|       |      |      |      |      |
|       |      |      |      |      |
|       |      |      |      |      |
|       |      |      |      |      |

