# 1

$$
\begin{align*}
{\rm set }&\\
& p = 2n+1,n\in \N\\
& q = 2m+1,m\in \N\\\\
\because\\
p+q &= (2n+1)+(2m+1)\\
&=2n+2m+2\\
&=2(n+m+1)\\
\therefore &{\rm\ sum\ of\ two\ odd\ intergers\ is\ even}
\end{align*}
$$

# 2

## a)

$$
\begin{align*}
\text{proof A: }&{\rm if\ }n{\rm\ is\ odd,}{\rm\ then\ }n^3+5{\rm\ is\ even}\\
&n= 2k+1,k\in \Z\\
&\because(2k+1)^3+5= 8k^3+12k^+6k+6=2(4k^3+6k^2+3k+3)  \\
&\therefore n^3+5\text{ is even}\\
&\therefore \text{if n is an interger and }n^3+5\text{ is odd, then }n\text{ is even.}
\end{align*}
$$

## b)

$$
\begin{align*}
\text{proof B: }&\text{if n in an integer and }n^3+5\text{ is odd, then }n\text{ is odd}\\
&\because n^3+5= 2p+1,k\in\Z;\ n=2q+1,q\in\Z \\
&\therefore n^3 = 2p= (2q+1)^3\\
&\because 2p\neq2(4q^3+6q^2+3q)+1\\
&\therefore \text{B is false}\\
&\therefore \text{if n is an interger and }n^3+5\text{ is odd, then }n\text{ is even.}
\end{align*}
$$

# 3

$$
\begin{align*}
\text{if }x\ge y:&\\
&min(x,y)=\frac{x+y-\vert x-y\vert}{2}=\frac{x+y-(x-y)}{2}=y\\
\text{if }x\le y:&\\
&min(x,y)=\frac{x+y-\vert x-y\vert}{2}=\frac{x+y+(x-y)}{2}=x\\
\therefore \text{proved}&
\end{align*}
$$

# 4

$$
\begin{align*}
\text{proof }A\and B:&\\
&A:\text{if }n=2p+1,\text{ then }n^2=2q+1;p,q\in \Z\\
&B:\text{if }n^2=2p+1,\text{ then }n=2q+1;p,q\in \Z\\
A:&\\
&\because n=2p+1,\therefore n^2=4p^2+4p+1=2q+1\\
&\because 2q+1=2(2p^2+2p)+1\\
&\because (2p^2+2p)\in\Z\\
&\therefore \text{A proved}\\
B:&\\
&\because n^2=2p+1,\therefore n^2=2p+1=4q^2+4q+1\\
&\because 2p+1=2(2q^2+2q)+1\\
&\because (2q^2+2q)\in\Z\\
&\therefore \text{B proved}\\
\because A\and B &\\
\therefore\text{ if n is} &\text{ an integer,then n is odd if and only if }{\rm n^2}\text{ is odd}
\end{align*}
$$

# 5

$$
\begin{align*}
\text{proof A:}&\text{ sum of an irrational number and a rational number is rational}\\
&\because\sqrt{2}+1\text{ is an irrational number}\\
&\therefore \text{A is false}\\
&\therefore \text{ sum of an irrational number and a rational number is irrational}
\end{align*}
$$

# 6

$$
\begin{align*}
\text{if }a\ge b\ge c:&\\
&\because min(b,c)=c,min(a,c)=c\\
&\because min(a,b)=b,min(b,c)=c\\
&\therefore min(a,min(b,c))=min(min(a,b),c)\\
\text{if }a\ge c\ge b:&\\
&\because min(b,c)=b,min(a,c)=b\\
&\because min(a,b)=b,min(b,c)=b\\
&\therefore min(a,min(b,c))=min(min(a,b),c)\\
\text{if }b\ge a\ge c:&\\
&\because min(b,c)=c,min(a,c)=c\\
&\because min(a,b)=a,min(b,c)=c\\
&\therefore min(a,min(b,c))=min(min(a,b),c)\\
\text{if }b\ge c\ge a:&\\
&\because min(b,c)=c,min(a,c)=a\\
&\because min(a,b)=a,min(b,c)=a\\
&\therefore min(a,min(b,c))=min(min(a,b),c)\\
\text{if }c\ge a\ge b:&\\
&\because min(b,c)=b,min(a,c)=b\\
&\because min(a,b)=b,min(b,c)=b\\
&\therefore min(a,min(b,c))=min(min(a,b),c)\\
\text{if }c\ge b\ge a:&\\
&\because min(b,c)=b,min(a,c)=a\\
&\because min(a,b)=a,min(b,c)=a\\
&\therefore min(a,min(b,c))=min(min(a,b),c)\\
\\
\text{Summarize }&\text{the above, }min(a,min(b,c))=min(min(a,b),c)\text{ is true}
\end{align*}
$$

# 7

$$
\begin{align*}
\text{Proof A: }&2^{\frac{1}{3}}\text{ is a rational number}\\
&\because 2^{\frac{1}{3}}\in\Q\\
&\therefore \text{set }2^{\frac1 3}=\frac{m}{n};m,n\in\Z,\frac{m}{n}\text{is simplified to lowest terms}\\
&\therefore (2^{\frac{1}{3}})^3=2=\frac{m^3}{n^3}\\
&\because m^3=2n^3\\
&\therefore m^3\text{ is even, }m\text{ is also even}\\
&\ \ \text{ let }m=2k, 2=\frac{(2k)^3}{n^3}\\
&\therefore 2=\frac{8k^3}{n^3}\\
&\therefore n^3=4k^3\\
&\therefore n^3\text{ is even, }n\text{ is also even}\\
&\because m,n\text{ are even and }\frac{m}{n}\text{ is simplified to lowest terms}\\
&\therefore A\text{ is false}\\
&\therefore 2^{\frac{1}{3}}\text{ is a irrational number}
\end{align*}
$$

# 8

  
$$
\begin{align*}
\text{When }n=1:&\\
&n^2+1=2,2^n=2\\
&n^2+1\geq2^n\\

\text{When }n=2:&\\
&n^2+1=5,2^n=4\\
&n^2+1\geq2^n\\

\text{When }n=3:&\\
&n^2+1=10,2^n=8\\
&n^2+1\geq2^n\\

\text{When }n=4:&\\
&n^2+1=17,2^n=16\\
&n^2+1\geq2^n\\
\therefore \text{When n is }&\text{integer and }1\leq n\leq4,\\& n^2+1\geq2
\end{align*}
$$




# 9

$$
\begin{align*}
\text{Proof A : }&\exist k_3\in\Z,(3k_1+1)(3k_2+2)=3k_3+2(k_1,k_2\in\Z)\\
&(3k_1+1)(3k_2+2)\\
&=9k_1k_2+6k_1+3k_2+2\\
&=3(3k_1k_2+2k_1+k_2)+2\\
&\because k_1,k_2\in\Z\\
&\therefore (3k_1k_2+2k_1+k_2)\in\Z\\
&\text{When }k_3=3k_1k_2+2k_1+k_2,\ (3k_1+1)(3k_2+2)=3k_3+2\\
&\therefore\text{A is true}
\end{align*}
$$

# 10

$$
\begin{align*}
(A\Delta B)&=(A\cup B)-(A\cap B)\\
&=(A-A\cap B)\cup(B-A\cap B)\\
&=(A-B)\cup(B-A)
\end{align*}
$$























