# Tutorial 5

## 1

### (i)

| x | -2 | -1 | 0 | 1 | 2 |
| - | -- | -- | - | - | - |
| f | 1  | 4  | 5 | 4 | 1 |

![T5\_1](assets/T5\_1\_i.png)

### (ii)

Not Injective

Surjective

### (iii)

no

### (iv)

| x | -2  | -1  | 0 | 1   | 2   |
| - | --- | --- | - | --- | --- |
| f | 0.6 | 0.8 | 1 | 1.2 | 1.4 |

![T5\_1\_iv](assets/T5\_1\_iv.png)

## 2

*   a

    Not injective

    Not surjective

    ![image-20221124192027202](assets/T5\_2\_a.png)
*   b

    Bijective

    ![image-20221124192123751](assets/T5\_2\_b.png)

## 3

### (i)

$$
\begin{align*} f\circ f=\\ &\{((a,b),(b,a)),((b,a),(a,b)),((c,b),(b,a))\} \end{align*}
$$

$$
\begin{align*} f\circ f\circ f= &\{\\ &(((a,b),(b,a)),((b,a),(a,b))),\\ &(((b,a),(a,b)),(a,b),(b,a))),\\ &(((c,b),(b,a)),((b,a),(a,b))),\\ &\} \end{align*}
$$

### (ii)

## 4

### (i)

2

### (ii)

\-10

### (iii)

\-3

### (iv)

4

## 5

### (i)

X : -2, -1, 0, 1, 2

Y : 0, 1, 2

### (ii)

|X|=5

|Y|=3

### (iii)

13

### (iv)

6

## 6

### (i)

$f^{-1}(y)=\sqrt{y}+3$

### (ii)

$f^{-1}(y)=\frac{2y-1}{1-y}$

### (iii)

$f^{-1}(y)=\sqrt y -1$

## 7

### (i)

$$
\begin{align*} f \circ g&=f(g(x))\\ &=2(-x^2+1)+3\\ &=-2x^2+5\\ \\ g\circ f&=g(f(x))\\ &=-(2x+3)^2+1\\ &=-4x^2-12x-8\\ \\ f\circ f&=f(f(x))\\ &=2(2x+3)+3\\ &=4x+9\\ \\ g\circ g&=g(g(x))\\ &=-(-x^2+1)^2+1\\ &=-x^4-2x^2 \end{align*}
$$

## 8

$f(x)=\frac{|x|}x$

## 9

![download](assets/T5\_9.png)

![image-20221124220915640](assets/T5\_9\(2\).png)

Not Injective, Not Surjective
